theories/typing/bitfield.v
@@ -115,8 +115,8 @@ Section programs.
   (* typing rules for bitfield_raw *)
 
   Lemma type_arithop_bitfield_raw it v1 bv1 v2 bv2 T bv op:
-    arith_op_result it bv1 bv2 op = Some bv →
-    (⌜bv1 ∈ it⌝ -∗ ⌜bv2 ∈ it⌝ -∗ ⌜arith_op_sidecond it bv1 bv2 bv op⌝ ∗
+    int_arithop_result it bv1 bv2 op = Some bv →
+    (⌜bv1 ∈ it⌝ -∗ ⌜bv2 ∈ it⌝ -∗ ⌜int_arithop_sidecond it bv1 bv2 bv op⌝ ∗
       (tactic_hint (normalize_bitfield bv) (λ norm, T (i2v norm it) (norm @ bitfield_raw it)))) -∗
     typed_bin_op v1 (v1 ◁ᵥ bv1 @ bitfield_raw it) v2 (v2 ◁ᵥ bv2 @ bitfield_raw it) op (IntOp it) (IntOp it) T.
   Proof.
@@ -191,8 +191,8 @@ Section programs.
   (* bitfield_raw with int *)
 
   Lemma type_arithop_bitfield_raw_int it v1 bv v2 n T bv' op:
-    arith_op_result it bv n op = Some bv' →
-    (⌜bv ∈ it⌝ -∗ ⌜n ∈ it⌝ -∗ ⌜arith_op_sidecond it bv n bv' op⌝ ∗
+    int_arithop_result it bv n op = Some bv' →
+    (⌜bv ∈ it⌝ -∗ ⌜n ∈ it⌝ -∗ ⌜int_arithop_sidecond it bv n bv' op⌝ ∗
       (tactic_hint (normalize_bitfield bv') (λ norm, T (i2v norm it) (norm @ bitfield_raw it)))) -∗
       typed_bin_op v1 (v1 ◁ᵥ bv @ bitfield_raw it) v2 (v2 ◁ᵥ n @ int it) op (IntOp it) (IntOp it) T.
   Proof.
@@ -212,8 +212,8 @@ Section programs.
   Next Obligation. done. Qed.
 
   Lemma type_arithop_int_bitfield_raw it v1 n v2 bv T bv' op:
-    arith_op_result it n bv op = Some bv' →
-    (⌜n ∈ it⌝ -∗ ⌜bv ∈ it⌝ -∗ ⌜arith_op_sidecond it n bv bv' op⌝ ∗
+    int_arithop_result it n bv op = Some bv' →
+    (⌜n ∈ it⌝ -∗ ⌜bv ∈ it⌝ -∗ ⌜int_arithop_sidecond it n bv bv' op⌝ ∗
       (tactic_hint (normalize_bitfield bv') (λ norm, T (i2v norm it) (norm @ bitfield_raw it)))) -∗
     typed_bin_op v1 (v1 ◁ᵥ n @ int it) v2 (v2 ◁ᵥ bv @ bitfield_raw it) op (IntOp it) (IntOp it) T.
   Proof.
